theories/progress.v
@@ -71,6 +71,45 @@ Lemma rtyped_inner e t :
 Proof.
   iIntros "H".
   iInduction e as [] "IH" forall (t); simpl; [eauto|eauto|..].
+  - iDestruct "H" as (t1 t2 ->) "[H1 H2]".
+    iDestruct ("IH" with "H1") as "%". iClear "IH".
+    iDestruct ("IH1" with "H2") as "%". iClear "IH1".
+    destruct H as [[v ->]|(k & e0 & Hk & -> & H)].
+    + destruct H0 as [[v' ->]|(k & e0 & Hk & -> & H0)].
+      * iPureIntro. right. exists (λ x, x). eexists.
+        split_and!; eauto.
+        { constructor. }
+        left. eexists.
+        constructor.
+      * iPureIntro. right.
+        eexists (λ x, Pair (Val v) (k x)),_.
+        split_and!; eauto.
+        constructor; eauto. constructor.
+    + iPureIntro. right.
+      eexists (λ x, Pair (k x) e2),_.
+      split_and!; eauto.
+      eapply (Ctx_cons (λ x, Pair x e2)); eauto. constructor.
+  (* - iDestruct "H" as (t1 t2 ->) "[H1 H2]".
+    iDestruct ("IH" with "H1") as "%". iClear "IH".
+    iDestruct ("IH1" with "H2") as "%". iClear "IH1".
+    destruct H as [[v ->]|(k & e0 & Hk & -> & H)].
+    + destruct H0 as [[v' ->]|(k & e0 & Hk & -> & H0)].
+      * simpl. rewrite val_typed_val_typed'. simpl.
+        iDestruct "H1" as (x e ->) "H1".
+        iPureIntro. right. exists (λ x, x). eexists.
+        split_and!; eauto.
+        { constructor. }
+        left. eexists.
+        constructor.
+      * iPureIntro. right.
+        eexists (λ x, App (Val v) (k x)),_.
+        split_and!; eauto.
+        constructor; eauto. constructor.
+    + iPureIntro. right.
+      eexists (λ x, App (k x) e2),_.
+      split_and!; eauto.
+      eapply (Ctx_cons (λ x, App x e2)); eauto.
+      constructor. *)
   - iDestruct "H" as (t') "[H1 H2]".
     iDestruct ("IH" with "H1") as "%". iClear "IH".
     iDestruct ("IH1" with "H2") as "%". iClear "IH1".
